refactoring...

VCVio/OracleComp/SimSemantics/SimulateQ.lean
@@ -3,7 +3,7 @@ Copyright (c) 2024 Devon Tuma. All rights reserved.
 Released under Apache 2.0 license as described in the file LICENSE.
 Authors: Devon Tuma
 -/
-import VCVio.OracleComp.DistSemantics.Support
+import VCVio.OracleComp.OracleComp
 import ToMathlib.Control.StateT
 
 /-!
@@ -47,10 +47,10 @@ section simulateQ
 /-- Canonical lifting of a function `OracleQuery spec α → m α`
 to a new function `OracleComp spec α` by preserving `bind`, `pure`, and `failure`.
 NOTE: could change the output type to `OracleComp spec →ᵐ m`, makes some stuff below free -/
-def simulateQ [AlternativeMonad m] [LawfulAlternative m]
-    (so : QueryImpl spec m) (oa : OracleComp spec α) : m α :=
-  OptionT.mapM' (FreeMonad.mapM' m so.impl) oa
+def simulateQ [AlternativeMonad m] (so : QueryImpl spec m) (oa : OracleComp spec α) : m α :=
+  OptionT.mapM (fun x => x.mapM so.impl) oa
 
+-- TODO: can remove `LawfulAlternative`s around a lot now.
 variable [AlternativeMonad m] [LawfulAlternative m] (so : QueryImpl spec m)
 
 @[simp]
@@ -59,16 +59,16 @@ lemma simulateQ_failure : simulateQ so (failure : OracleComp spec α) = failure 
 
 @[simp]
 lemma simulateQ_query (q : OracleQuery spec α) : simulateQ so q = so.impl q := by
-  simp [simulateQ, OracleComp.liftM_def]
+  sorry --simp [simulateQ, OracleComp.liftM_def]
 
 @[simp]
 lemma simulateQ_pure (x : α) : simulateQ so (pure x) = pure x :=
-  MonadHom.mmap_pure _ x
+  sorry --MonadHom.mmap_pure _ x
 
 @[simp]
 lemma simulateQ_bind (oa : OracleComp spec α) (ob : α → OracleComp spec β) :
     simulateQ so (oa >>= ob) = simulateQ so oa >>= fun x => simulateQ so (ob x) :=
-  MonadHom.mmap_bind _ oa ob
+  sorry --MonadHom.mmap_bind _ oa ob
 
 @[simp]
 lemma simulateQ_map (oa : OracleComp spec α) (f : α → β) :
@@ -93,165 +93,11 @@ lemma simulateQ_ite (p : Prop) [Decidable p] (oa oa' : OracleComp spec α) :
 
 end simulateQ
 
-section simulate
-
-/-- `simulate so oa s` runs the computation `oa`, using the simulation oracle `so` to
-answer any queries to the oracle, starting the simulation oracle's state with `s`.
-TODO: deprecate -/
-@[reducible]
-def simulate (so : QueryImpl spec (StateT σ (OracleComp specₜ))) (s : σ)
-    (oa : OracleComp spec α) : OracleComp specₜ (α × σ) :=
-  (simulateQ so oa).run s
-
-/-- Version of `simulate` that tosses out the oracle state at the end. -/
-@[reducible]
-def simulate' (so : QueryImpl spec (StateT σ (OracleComp specₜ))) (s : σ)
-    (oa : OracleComp spec α) : OracleComp specₜ α :=
-  (simulateQ so oa).run' s
-
-variable (so : QueryImpl spec (StateT σ (OracleComp specₜ)))
-
-lemma simulate_def (s : σ) (oa : OracleComp spec α) :
-    simulate so s oa = (simulateQ so oa).run s := rfl
-
-lemma simulate'_def (s : σ) (oa : OracleComp spec α) :
-    simulate' so s oa = (simulateQ so oa).run' s := rfl
-
-section basic
-
-@[simp low]
-lemma simulate_pure (s : σ) (x : α) : simulate so s (pure x) = pure (x, s) := rfl
-
-@[simp low]
-lemma simulate'_pure (s : σ) (x : α) : simulate' so s (pure x) = pure x := rfl
-
-@[simp]
-lemma simulate_failure (s : σ) : simulate so s (failure : OracleComp spec α) = failure := rfl
-
-@[simp]
-lemma simulate'_failure (s : σ) : simulate' so s (failure : OracleComp spec α) = failure := rfl
-
-@[simp low]
-lemma simulate_bind (s : σ)  (oa : OracleComp spec α) (ob : α → OracleComp spec β) :
-    (simulate so s (oa >>= ob) = do let z ← simulate so s oa; simulate so z.2 (ob z.1)) := by
-  simp [simulate, simulateQ_bind, StateT.run_bind]
-
-@[simp low]
-lemma simulate'_bind (s : σ) (oa : OracleComp spec α) (ob : α → OracleComp spec β) :
-    (simulate' so s (oa >>= ob) = do let z ← simulate so s oa; simulate' so z.2 (ob z.1)) := by
-  simp [simulate', simulate]
-
-@[simp low]
-lemma simulate_query (s : σ) (q : OracleQuery spec α) :
-    simulate so s q = (so.impl q).run s := by
-  simp [simulate', simulate]
-
-@[simp low]
-lemma simulate'_query (s : σ) (q : OracleQuery spec α) :
-    simulate' so s q = (so.impl q).run' s := by
-  simp [simulate']
-
-lemma simulate_query_bind (s : σ) (q : OracleQuery spec β)
-    (oa : β → OracleComp spec α) : simulate so s (q >>= oa) =
-    (do let (u, s') ← (so.impl q).run s; simulate so s' (oa u)) := by
-  rw [simulate_bind, simulate_query]
-
-lemma simulate'_query_bind (s : σ) (q : OracleQuery spec β)
-    (oa : β → OracleComp spec α) : simulate' so s (q >>= oa) =
-    (do let (u, s') ← (so.impl q).run s; simulate' so s' (oa u)) := by
-  rw [simulate'_bind, simulate_query]
-
-@[simp low]
-lemma simulate_map (s : σ) (oa : OracleComp spec α) (f : α → β) :
-    simulate so s (f <$> oa) = (map f id) <$> simulate so s oa := by
-  simp [simulate, map]; rfl
-
-@[simp low]
-lemma simulate'_map (s : σ) (oa : OracleComp spec α) (f : α → β) :
-    simulate' so s (f <$> oa) = f <$> simulate' so s oa := by
-  simp [simulate']
-
-@[simp low]
-lemma simulate_seq (s : σ) (oa : OracleComp spec α) (og : OracleComp spec (α → β)) :
-    simulate so s (og <*> oa) = simulate so s og >>= λ z ↦
-      (map z.1 id <$> simulate so z.2 oa) := by
-  simp [seq_eq_bind]
-
-@[simp low]
-lemma simulate'_seq (s : σ) (oa : OracleComp spec α) (og : OracleComp spec (α → β)) :
-    simulate' so s (og <*> oa) = simulate so s og >>= λ z ↦
-      (z.1 <$> simulate' so z.2 oa) := by
-  simp [simulate']
-
-end basic
-
-section support
-
-lemma support_simulate' (oa : OracleComp spec α) (s : σ) :
-    (simulate' so s oa).support = fst <$> (simulate so s oa).support :=
-  support_map _ fst
-
-/-- Since `support` assumes any possible query result, `simulate` will never reduce the support.
-In particular the support of a simulation lies in the preimage of the original support. -/
-lemma support_simulate_subset_preimage_support (oa : OracleComp spec α) (s : σ) :
-    (simulate so s oa).support ⊆ fst ⁻¹' oa.support := by
-  revert s
-  induction oa using OracleComp.inductionOn with
-  | pure x => simp
-  | query_bind i t oa hoa =>
-      simp [hoa]
-      refine λ _ t s' _ ↦ Set.subset_iUnion_of_subset t (hoa t s')
-  | failure => simp
-
-/-- Simulation only reduces the possible oracle outputs, so can't reduce the support. In particular
-the first output of a simulation has support at most that of the original computation -/
-lemma support_simulate'_subset_support (oa : OracleComp spec α) (s : σ) :
-    (simulate' so s oa).support ⊆ oa.support := by
-  rw [simulate', StateT.run', support_map, Set.image_subset_iff]
-  apply support_simulate_subset_preimage_support
-
-lemma mem_support_simulate'_of_mem_support_simulate {oa : OracleComp spec α} {s : σ} {x : α}
-    (s' : σ) (h : (x, s') ∈ (simulate so s oa).support) : x ∈ (simulate' so s oa).support := by
-  simp only [support_simulate', Set.fmap_eq_image, Set.mem_image, Prod.exists, exists_and_right,
-    exists_eq_right]
-  exact ⟨s', h⟩
-
-end support
-
 section subsingleton
 
-variable {σ : Type u} [Subsingleton σ] (so : QueryImpl spec (StateT σ (OracleComp specₜ)))
 
-/-- If the state type is `Subsingleton`, then we can represent simulation in terms of `simulate'`,
-adding back any state at the end of the computation. -/
-lemma simulate_eq_map_simulate'_of_subsingleton (oa : OracleComp spec α) (s s' : σ) :
-    simulate so s oa = (·, s') <$> simulate' so s oa := by
-  have : (λ x : α × σ ↦ (x.1, s')) = id :=
-    funext λ (x, s) ↦ Prod.eq_iff_fst_eq_snd_eq.2 ⟨rfl, Subsingleton.elim _ _⟩
-  simp [simulate', simulate, this]
-
-lemma simulate_eq_map_simulate' [Inhabited σ] (oa : OracleComp spec α) (s : σ) :
-    simulate so s oa = (·, default) <$> simulate' so s oa :=
-  simulate_eq_map_simulate'_of_subsingleton so oa s default
 
 end subsingleton
-
-end simulate
-
-section support_test
-
-variable {ι : Type u} {spec : OracleSpec ι} {α : Type v}
-
-attribute [local instance] Set.monad
-
-def supportWhen' (ox : OracleComp spec α)
-    (possible_outputs : {α : Type v} → OracleQuery spec α → Set α) : Set α :=
-  ox.simulateQ ⟨possible_outputs⟩
-
-def support' (oa : OracleComp spec α) : Set α :=
-  oa.simulateQ ⟨fun | query i _ => Set.univ⟩
-
-end support_test
 
 end OracleComp
 
