VCVio/OracleComp/Constructions/GenerateSeed.lean
@@ -3,7 +3,7 @@ Copyright (c) 2024 Devon Tuma. All rights reserved.
 Released under Apache 2.0 license as described in the file LICENSE.
 Authors: Devon Tuma
 -/
-import VCVio.OracleComp.SimSemantics.QueryTracking.SeededOracle
+import VCVio.OracleComp.QueryTracking.SeededOracle
 import VCVio.OracleComp.Constructions.Replicate
 import VCVio.OracleComp.Constructions.UniformSelect
 import Mathlib.Data.List.Basic
