VCVio/OracleComp/QueryTracking/CachingOracle.lean
@@ -3,7 +3,7 @@ Copyright (c) 2024 Devon Tuma. All rights reserved.
 Released under Apache 2.0 license as described in the file LICENSE.
 Authors: Devon Tuma
 -/
-import VCVio.OracleComp.SimSemantics.QueryTracking.Structures
+import VCVio.OracleComp.QueryTracking.Structures
 import VCVio.OracleComp.SimSemantics.Constructions
 
 /-!
