VCVio/OracleComp/QueryTracking/SeededOracle.lean
@@ -4,7 +4,7 @@ Released under Apache 2.0 license as described in the file LICENSE.
 Authors: Devon Tuma
 -/
 import VCVio.OracleComp.SimSemantics.Constructions
-import VCVio.OracleComp.SimSemantics.QueryTracking.Structures
+import VCVio.OracleComp.QueryTracking.Structures
 
 /-!
 # Pre-computing Results of Oracle Queries
