VCVio/OracleComp/Traversal.lean
@@ -1,0 +1,120 @@
+/-
+Copyright (c) 2024 Devon Tuma. All rights reserved.
+Released under Apache 2.0 license as described in the file LICENSE.
+Authors: Devon Tuma
+-/
+import VCVio.OracleComp.Support
+
+/-!
+# Traversing Possible Paths of a Computation.
+
+This file defines functions `alwaysWhen` and `someWhen` that allow for traversing a computation's
+structure to check some given predicates on each node, using a set of possible outputs for that
+traversal. These definitions are `Prop` not `Bool` and should usually only be used in proofs,
+not in defining an actual computaion.
+
+The file also contains many special cases of these functions like `neverFailsWhen`.
+
+-/
+
+open OracleSpec
+
+universe u v w
+
+namespace OracleComp
+
+variable {ι : Type u} {spec : OracleSpec ι} {α β γ : Type v}
+
+section allWhen
+
+variable
+    (query_pred : {α : Type v} → OracleQuery spec α → Prop)
+    (fail_pred : Prop) (oa : OracleComp spec α)
+    (possible_outputs : {α : Type v} → OracleQuery spec α → Set α)
+
+/-- All the given predicates hold on a computation when queries respond with
+elements of `possible_outputs q` for every query `q` -/
+def allWhen (possible_outputs : {α : Type v} → OracleQuery spec α → Set α)
+    (oa : OracleComp spec α) : Prop := by
+  induction oa using OracleComp.construct with
+  | pure x => exact True
+  | failure => exact fail_pred
+  | query_bind q _ r => exact query_pred q ∧ ∀ x ∈ possible_outputs q, r x
+
+@[simp] lemma allWhen_pure (x : α) : (pure x : OracleComp spec α).allWhen
+     query_pred fail_pred possible_outputs := True.intro
+
+@[simp] lemma allWhen_failure_iff : (failure : OracleComp spec α).allWhen
+   query_pred fail_pred possible_outputs ↔ fail_pred := Iff.rfl
+
+@[simp] lemma allWhen_query_iff (q : OracleQuery spec α) : (q : OracleComp spec α).allWhen
+    query_pred fail_pred possible_outputs ↔ query_pred q := by simp [allWhen]
+
+@[simp] lemma allWhen_query_bind (q : OracleQuery spec α) (oa : α → OracleComp spec β) :
+    ((q : OracleComp spec α) >>= oa).allWhen query_pred fail_pred possible_outputs ↔ query_pred q ∧
+      ∀ x ∈ possible_outputs q, (oa x).allWhen query_pred fail_pred possible_outputs := by rfl
+
+-- TODO: We need a full theory of `supportWhen` to make this work well.
+-- @[simp] lemma allWhen_bind_iff (oa : OracleComp spec α) (ob : α → OracleComp spec β) :
+--     (oa >>= ob).allWhen query_pred fail_pred possible_outputs ↔
+--       oa.allWhen query_pred fail_pred possible_outputs ∧
+--         ∀ x ∈ oa.supportWhen possible_outputs, (ob x).allWhen query_pred fail_pred possible_outputs := by
+--   induction oa using OracleComp.inductionOn with
+--   | pure x => {
+--     simp [supportWhen]
+--   }
+--   | failure => {
+--     simp [supportWhen]
+--   }
+--   | query_bind i t oa h => {
+--     rw [bind_assoc, allWhen_query_bind]
+--     simp [h, supportWhen]
+--     rw [and_assoc]
+--     refine and_congr_right fun _ => ?_
+--   }
+
+end allWhen
+
+variable (pure_pred : {α : Type v} → α → Prop)
+    (query_pred : {α : Type v} → OracleQuery spec α → Prop)
+    (fail_pred : Prop) (oa : OracleComp spec α)
+    (possible_outputs : {α : Type v} → OracleQuery spec α → Set α)
+
+/-- One of the given predicates hold on a computation when queries respond with
+elements of `possible_outputs q` for every query `q` -/
+def someWhen (possible_outputs : {α : Type v} → OracleQuery spec α → Set α)
+    (oa : OracleComp spec α) : Prop := by
+  induction oa using OracleComp.construct with
+  | pure x => exact pure_pred x
+  | failure => exact fail_pred
+  | query_bind q _ r => exact query_pred q ∨ ∃ x ∈ possible_outputs q, r x
+
+section neverFail
+
+/-- `oa` never fails if when responses to queries `q` are in `possible_outputs q`. -/
+def neverFailWhen (oa : OracleComp spec α)
+    (possible_outputs : {α : Type v} → OracleQuery spec α → Set α) : Prop :=
+  oa.allWhen (fun _ => True) False possible_outputs
+
+/-- `oa` never fails even when queries can output any possible value. -/
+@[reducible, inline] def neverFail (oa : OracleComp spec α) : Prop :=
+  oa.neverFailWhen fun _ => Set.univ
+
+end neverFail
+
+section mayFail
+
+/-- `oa` might fail when responses to queries `q` are in `possible_outputs q`-/
+def mayFailWhen (oa : OracleComp spec α)
+    (possible_outputs : {α : Type v} → OracleQuery spec α → Set α) : Prop :=
+  oa.someWhen (fun _ => False) (fun _ => False) True possible_outputs
+
+-- lemma mayFailWhen_iff_not_neverFailWhen
+
+/-- `oa` might fail if queries can output any possible value. -/
+@[reducible, inline] def mayFail (oa : OracleComp spec α) : Prop :=
+  mayFailWhen oa fun _ => Set.univ
+
+end mayFail
+
+end OracleComp
